Start work on proving kernel is normal

Groups1stIso/Homomorphism/Defs.lean
@@ -35,36 +35,53 @@ variable {G H : Type _} [MyGroup G] [MyGroup H]
 variable (f : G → H) [MyGroupHom f]
 
 
+-- Kernel of a group homomorphism is a subgroup
+instance Myker_is_subgroup :
+  MySubgroup G (Myker f) := by
+  constructor
+  · refine Set.mem_preimage.mpr ?_
+    have : f (1 : G) = 1 := MyGroupHom.hom_id
+    exact this
+  · intro a b h
+    obtain ⟨ha, hb⟩ := h
+    refine Set.mem_preimage.mpr ?_
+    have : f (a * b) = f a * f b := MyGroupHom.hom_mul a b
+    rw [this, ha, hb, MyGroup.one_mul]
+    rfl
+  · intro a ha
+    refine Set.mem_preimage.mpr ?_
+    have : f (a⁻¹) = (f a)⁻¹ := MyGroupHom.hom_inv a
+    rw [this, ha, OurGroupProp.one_inv (G := H)]
+    rfl
+
 -- Kernel of a group homomorphism is a normal subgroup
 instance Myker_is_normal :
   NormalSubgroup G (Myker f) := by
   constructor
-  · refine { identity := ?_, mul_closed := ?_, inv_closed := ?_ }
-    · refine Set.mem_preimage.mpr ?_
-      have : f (1 : G) = 1 := MyGroupHom.hom_id
-      exact this
-    · intro a b h
-      obtain ⟨ha, hb⟩ := h
-      refine Set.mem_preimage.mpr ?_
-      have : f (a * b) = f a * f b := MyGroupHom.hom_mul a b
-      rw [this, ha, hb, MyGroup.one_mul]
-      rfl
-    · intro a ha
-      refine Set.mem_preimage.mpr ?_
-      have : f (a⁻¹) = (f a)⁻¹ := MyGroupHom.hom_inv a
-      rw [this]
-      rw [ha]
-      
-      sorry
-  · sorry
+  · exact Myker_is_subgroup f
+  · intro g h
+    refine Set.mem_preimage.mpr ?_
+    have : f (g * h * g⁻¹) = f g * f h * (f g)⁻¹ := by
+      simp only [MyGroupHom.hom_mul, MyGroupHom.hom_inv, MyGroup.one_mul]
+    rw [this]
+    have : f h = 1 := by
+      have h_in_ker := h.property
+      simp only [Myker, Set.mem_preimage, Set.mem_singleton_iff] at h_in_ker
+      exact h_in_ker
+    rw [this]
+    simp only [MyGroup.one_mul, MyGroup.mul_one]
+    rw [MyGroup.mul_right_inv]
+    rfl
+
 
 -- Image of a group homomorphism is a group
 instance Myim_is_group :
-  MyGroup (Myim f) := by sorry
+  MyGroup (Myim f) := by
+  sorry
 
 -- The first isomorphism theorem
 theorem FirstIsoTheorem :
   ∃ φ : MyQuotientGroup (Myker_is_normal f) → Myim f,
     MyGroupIso φ := by sorry
-
+    
 end OurFirstIso
