Groups1stIso/1stIso.lean
@@ -1,0 +1,2 @@
+import Groups1stIso.Groups.Basics
+import Groups1stIso.Groups.Thms
